thys/Core_DOM/common/monads/BaseMonad.thy
@@ -36,8 +36,8 @@ theory BaseMonad
 begin
 subsection\<open>Datatypes\<close>
 
-datatype exception = NotFoundError | SegmentationFault | HierarchyRequestError | AssertException 
-  | NonTerminationException | InvokeError | TypeError | DebugException nat
+datatype exception = NotFoundError | HierarchyRequestError | NotSupportedError | SegmentationFault
+  | AssertException | NonTerminationException | InvokeError | TypeError
 
 lemma finite_set_in [simp]: "x \<in> fset FS \<longleftrightarrow> x |\<in>| FS"
   by (meson notin_fset)
@@ -150,7 +150,7 @@ proof (unfold comp_def, rule ccpo.admissibleI, clarify)
     by (rule chain_fun[OF 1])
   show "P h h2 r"
     using chain_fun[OF 1] flat_lub_in_chain[OF chain_fun[OF 1]] 2 4 unfolding execute_def fun_lub_def
-    by auto (metis (lifting) Inl_Inr_False)
+    by force
 qed
 
 lemma execute_admissible2: 
@@ -171,17 +171,18 @@ proof (unfold comp_def, rule ccpo.admissibleI, clarify)
   have "h \<turnstile> ?lub \<in> {y. \<exists>f\<in>A. y = f h}"
     using flat_lub_in_chain[OF h1] 4
     unfolding execute_def fun_lub_def
-    by auto (metis (lifting) Inl_Inr_False)
+    by auto
   moreover have "h' \<turnstile> ?lub \<in> {y. \<exists>f\<in>A. y = f h'}"
     using flat_lub_in_chain[OF h1] 5
     unfolding execute_def fun_lub_def
-    by auto (metis (lifting) Inl_Inr_False)
+    by auto
   ultimately obtain f where
     "f \<in> A" and
     "h \<turnstile> Prog f = Inr (r, h2)" and
     "h' \<turnstile> Prog f = Inr (r', h2')"
     using 1 4 5 
-    by (auto simp add: chain_def fun_ord_def flat_ord_def execute_def)[1] (metis (lifting) Inl_Inr_False)
+    apply(auto simp add:  chain_def fun_ord_def flat_ord_def execute_def)[1]
+    by (metis Inl_Inr_False)
   then show "P h h' h2 h2' r r'"
     by(fact 2)
 qed
