thys/Core_DOM/common/monads/DocumentMonad.thy
@@ -322,7 +322,8 @@ lemma type_wf_put_ptr_in_heap_E:
   using assms
   apply(auto simp add: type_wf_defs elim!: CharacterDataMonad.type_wf_put_ptr_in_heap_E 
       split: option.splits if_splits)[1]
-  by (metis (no_types, lifting) CharacterDataClass.get\<^sub>O\<^sub>b\<^sub>j\<^sub>e\<^sub>c\<^sub>t_type_wf bind.bind_lunit get\<^sub>D\<^sub>o\<^sub>c\<^sub>u\<^sub>m\<^sub>e\<^sub>n\<^sub>t_def is_document_kind_def notin_fset option.exhaust_sel)
+  by (metis (no_types, lifting) CharacterDataClass.get\<^sub>O\<^sub>b\<^sub>j\<^sub>e\<^sub>c\<^sub>t_type_wf bind.bind_lunit get\<^sub>D\<^sub>o\<^sub>c\<^sub>u\<^sub>m\<^sub>e\<^sub>n\<^sub>t_def
+      is_document_kind_def notin_fset option.exhaust_sel)
 
 
 
@@ -347,8 +348,8 @@ lemma new_element_is_l_new_element [instances]:
   using l_new_element.intro new_element_type_wf_preserved
   by blast
 
-lemma put_M\<^sub>E\<^sub>l\<^sub>e\<^sub>m\<^sub>e\<^sub>n\<^sub>t_tag_type_type_wf_preserved [simp]: 
-  "h \<turnstile> put_M element_ptr tag_type_update v \<rightarrow>\<^sub>h h' \<Longrightarrow> type_wf h = type_wf h'"
+lemma put_M\<^sub>E\<^sub>l\<^sub>e\<^sub>m\<^sub>e\<^sub>n\<^sub>t_tag_name_type_wf_preserved [simp]:
+  "h \<turnstile> put_M element_ptr tag_name_update v \<rightarrow>\<^sub>h h' \<Longrightarrow> type_wf h = type_wf h'"
   apply(auto simp add: ElementMonad.put_M_defs put\<^sub>E\<^sub>l\<^sub>e\<^sub>m\<^sub>e\<^sub>n\<^sub>t_def put\<^sub>N\<^sub>o\<^sub>d\<^sub>e_def 
       DocumentClass.type_wf\<^sub>C\<^sub>h\<^sub>a\<^sub>r\<^sub>a\<^sub>c\<^sub>t\<^sub>e\<^sub>r\<^sub>D\<^sub>a\<^sub>t\<^sub>a DocumentClass.type_wf\<^sub>E\<^sub>l\<^sub>e\<^sub>m\<^sub>e\<^sub>n\<^sub>t
       DocumentClass.type_wf\<^sub>N\<^sub>o\<^sub>d\<^sub>e DocumentClass.type_wf\<^sub>O\<^sub>b\<^sub>j\<^sub>e\<^sub>c\<^sub>t
@@ -360,7 +361,9 @@ lemma put_M\<^sub>E\<^sub>l\<^sub>e\<^sub>m\<^sub>e\<^sub>n\<^sub>t_tag_type_typ
   apply(auto simp add: is_node_kind_def type_wf_defs ElementClass.type_wf_defs NodeClass.type_wf_defs
       ElementMonad.get_M_defs ObjectClass.type_wf_defs
       CharacterDataClass.type_wf_defs split: option.splits)[1]
-  apply (metis NodeClass.a_type_wf_def NodeClass.get\<^sub>N\<^sub>o\<^sub>d\<^sub>e_type_wf ObjectClass.a_type_wf_def bind.bind_lzero finite_set_in get\<^sub>E\<^sub>l\<^sub>e\<^sub>m\<^sub>e\<^sub>n\<^sub>t_def l_type_wf_def\<^sub>N\<^sub>o\<^sub>d\<^sub>e.a_type_wf_def option.collapse option.distinct(1) option.simps(3))
+   apply (metis NodeClass.a_type_wf_def NodeClass.get\<^sub>N\<^sub>o\<^sub>d\<^sub>e_type_wf ObjectClass.a_type_wf_def
+      bind.bind_lzero finite_set_in get\<^sub>E\<^sub>l\<^sub>e\<^sub>m\<^sub>e\<^sub>n\<^sub>t_def l_type_wf_def\<^sub>N\<^sub>o\<^sub>d\<^sub>e.a_type_wf_def option.collapse
+      option.distinct(1) option.simps(3))
   by (metis fmember.rep_eq)
 
 lemma put_M\<^sub>E\<^sub>l\<^sub>e\<^sub>m\<^sub>e\<^sub>n\<^sub>t_child_nodes_type_wf_preserved [simp]: 
@@ -376,7 +379,9 @@ lemma put_M\<^sub>E\<^sub>l\<^sub>e\<^sub>m\<^sub>e\<^sub>n\<^sub>t_child_nodes_
   apply(auto simp add: is_node_kind_def type_wf_defs ElementClass.type_wf_defs
       NodeClass.type_wf_defs ElementMonad.get_M_defs ObjectClass.type_wf_defs 
       CharacterDataClass.type_wf_defs split: option.splits)[1]
-  apply (metis NodeClass.a_type_wf_def NodeClass.get\<^sub>N\<^sub>o\<^sub>d\<^sub>e_type_wf ObjectClass.a_type_wf_def bind.bind_lzero finite_set_in get\<^sub>E\<^sub>l\<^sub>e\<^sub>m\<^sub>e\<^sub>n\<^sub>t_def l_type_wf_def\<^sub>N\<^sub>o\<^sub>d\<^sub>e.a_type_wf_def option.collapse option.distinct(1) option.simps(3))
+   apply (metis NodeClass.a_type_wf_def NodeClass.get\<^sub>N\<^sub>o\<^sub>d\<^sub>e_type_wf ObjectClass.a_type_wf_def
+      bind.bind_lzero finite_set_in get\<^sub>E\<^sub>l\<^sub>e\<^sub>m\<^sub>e\<^sub>n\<^sub>t_def l_type_wf_def\<^sub>N\<^sub>o\<^sub>d\<^sub>e.a_type_wf_def option.collapse
+      option.distinct(1) option.simps(3))
   by (metis fmember.rep_eq)
 
 lemma put_M\<^sub>E\<^sub>l\<^sub>e\<^sub>m\<^sub>e\<^sub>n\<^sub>t_attrs_type_wf_preserved [simp]: 
@@ -392,7 +397,9 @@ lemma put_M\<^sub>E\<^sub>l\<^sub>e\<^sub>m\<^sub>e\<^sub>n\<^sub>t_attrs_type_w
   apply(auto simp add: is_node_kind_def type_wf_defs ElementClass.type_wf_defs
       NodeClass.type_wf_defs ElementMonad.get_M_defs ObjectClass.type_wf_defs 
       CharacterDataClass.type_wf_defs split: option.splits)[1]
-  apply (metis NodeClass.a_type_wf_def NodeClass.get\<^sub>N\<^sub>o\<^sub>d\<^sub>e_type_wf ObjectClass.a_type_wf_def bind.bind_lzero finite_set_in get\<^sub>E\<^sub>l\<^sub>e\<^sub>m\<^sub>e\<^sub>n\<^sub>t_def l_type_wf_def\<^sub>N\<^sub>o\<^sub>d\<^sub>e.a_type_wf_def option.collapse option.distinct(1) option.simps(3))
+   apply (metis NodeClass.a_type_wf_def NodeClass.get\<^sub>N\<^sub>o\<^sub>d\<^sub>e_type_wf ObjectClass.a_type_wf_def
+      bind.bind_lzero finite_set_in get\<^sub>E\<^sub>l\<^sub>e\<^sub>m\<^sub>e\<^sub>n\<^sub>t_def l_type_wf_def\<^sub>N\<^sub>o\<^sub>d\<^sub>e.a_type_wf_def option.collapse
+      option.distinct(1) option.simps(3))
   by (metis fmember.rep_eq)
 
 lemma put_M\<^sub>E\<^sub>l\<^sub>e\<^sub>m\<^sub>e\<^sub>n\<^sub>t_shadow_root_opt_type_wf_preserved [simp]:
@@ -408,7 +415,9 @@ lemma put_M\<^sub>E\<^sub>l\<^sub>e\<^sub>m\<^sub>e\<^sub>n\<^sub>t_shadow_root_
   apply(auto simp add: is_node_kind_def type_wf_defs ElementClass.type_wf_defs
       NodeClass.type_wf_defs ElementMonad.get_M_defs ObjectClass.type_wf_defs 
       CharacterDataClass.type_wf_defs split: option.splits)[1]
-  apply (metis NodeClass.a_type_wf_def NodeClass.get\<^sub>N\<^sub>o\<^sub>d\<^sub>e_type_wf ObjectClass.a_type_wf_def bind.bind_lzero finite_set_in get\<^sub>E\<^sub>l\<^sub>e\<^sub>m\<^sub>e\<^sub>n\<^sub>t_def l_type_wf_def\<^sub>N\<^sub>o\<^sub>d\<^sub>e.a_type_wf_def option.collapse option.distinct(1) option.simps(3))
+   apply (metis NodeClass.a_type_wf_def NodeClass.get\<^sub>N\<^sub>o\<^sub>d\<^sub>e_type_wf ObjectClass.a_type_wf_def
+      bind.bind_lzero finite_set_in get\<^sub>E\<^sub>l\<^sub>e\<^sub>m\<^sub>e\<^sub>n\<^sub>t_def l_type_wf_def\<^sub>N\<^sub>o\<^sub>d\<^sub>e.a_type_wf_def option.collapse
+      option.distinct(1) option.simps(3))
   by (metis fmember.rep_eq)
 
 lemma new_character_data_type_wf_preserved [simp]: 
@@ -458,7 +467,8 @@ lemma new_document_type_wf_preserved [simp]: "h \<turnstile> new_document \<righ
       split: option.splits)[1]
   using document_ptrs_def apply fastforce
    apply (simp add: is_document_kind_def)
-  apply (metis Suc_n_not_le_n document_ptr.sel(1) document_ptrs_def fMax_ge ffmember_filter fimage_eqI is_document_ptr_ref)
+  apply (metis Suc_n_not_le_n document_ptr.sel(1) document_ptrs_def fMax_ge ffmember_filter
+      fimage_eqI is_document_ptr_ref)
   done
 
 locale l_new_document = l_type_wf +
@@ -498,7 +508,7 @@ lemma put_M\<^sub>D\<^sub>o\<^sub>c\<^sub>u\<^sub>m\<^sub>e\<^sub>n\<^sub>t_doct
   apply(auto simp add: is_document_kind_def type_wf_defs ElementClass.type_wf_defs 
       NodeClass.type_wf_defs ElementMonad.get_M_defs ObjectClass.type_wf_defs 
       CharacterDataClass.type_wf_defs split: option.splits)[1]
-  apply(auto simp add: get_M_defs)
+  apply(auto simp add: get_M_defs)[1]
   by (metis (mono_tags) error_returns_result finite_set_in option.exhaust_sel option.simps(4))
 
 lemma put_M\<^sub>D\<^sub>o\<^sub>c\<^sub>u\<^sub>m\<^sub>e\<^sub>n\<^sub>t_document_element_type_wf_preserved [simp]: 
@@ -599,5 +609,6 @@ lemma type_wf_drop: "type_wf h \<Longrightarrow> type_wf (Heap (fmdrop ptr (the_
   apply(auto simp add: type_wf_defs)[1]
   using type_wf_drop
    apply blast
-  by (metis (no_types, lifting) CharacterDataClass.get\<^sub>O\<^sub>b\<^sub>j\<^sub>e\<^sub>c\<^sub>t_type_wf CharacterDataMonad.type_wf_drop document_ptr_kinds_commutes finite_set_in fmlookup_drop get\<^sub>D\<^sub>o\<^sub>c\<^sub>u\<^sub>m\<^sub>e\<^sub>n\<^sub>t_def get\<^sub>O\<^sub>b\<^sub>j\<^sub>e\<^sub>c\<^sub>t_def heap.sel)
+  by (metis (no_types, lifting) CharacterDataClass.get\<^sub>O\<^sub>b\<^sub>j\<^sub>e\<^sub>c\<^sub>t_type_wf CharacterDataMonad.type_wf_drop
+      document_ptr_kinds_commutes finite_set_in fmlookup_drop get\<^sub>D\<^sub>o\<^sub>c\<^sub>u\<^sub>m\<^sub>e\<^sub>n\<^sub>t_def get\<^sub>O\<^sub>b\<^sub>j\<^sub>e\<^sub>c\<^sub>t_def heap.sel)
 end
